\documentclass[12pt]{article}
\usepackage[top=2cm, left=2cm,right=3cm,bottom=2cm]{geometry}
\usepackage{amsmath, amssymb}
\usepackage{url,enumerate, ifthen}
\newboolean{answers}
%\setboolean{answers}{true}  % set to true to include TODO statements
\setboolean{answers}{false}  % set to false to use input statements
%% USAGE:
%% \ifthenelse{\boolean{answers}}{\smallskip {\bf Answer:} (c). \newpage}{\newpage}

%\usepackage{tikz}

\newcommand\probskip{\vskip4cm}

\begin{document}
\pagestyle{empty}


\noindent Math 165 Midterm Exam \hskip1cm Section:\underline{\phantom{XXXXXX}} \hfill Name:\underline{\phantom{XXXXXXXXXX}}

\bigskip

{\bf Part A: Pencil \& Paper Only}

\bigskip

\noindent This part of the exam has 10 problems on 3 pages. Each problem is worth 5 points. You
may NOT use a calculator on this section. You must show all work. This part of the exam
will be collected after 45 minutes.

\begin{enumerate}
% 1
\item 
Find $dy/dx$ if
\[
y = \frac{3x^3}{5x^2 + 2}.
\]
You do not need to simplify your answer.

\medskip

\noindent {\bf Solution:}

\[
\frac{dy}{dx} = \frac{(9x^2)(5x^2 + 2) - (3x^3)(10x)}{(5x^2+2)^2}
\]

\medskip

% 2
\item
Suppose 
\[
g(x) = \frac{2}{x^2}.
\]
Find $g''(2)$. Simplify your answer.

\medskip
\noindent {\bf Solution:}
\[
g'(x) = -\frac{4}{x^3}
\qquad
g''(x) = \frac{12}{x^4}
\qquad
g''(2) = \frac{3}{4}
\]
\bigskip

\item If 
\[
y = t^3 \ln t
\]
find $dy/dt$. Simplify your answer.

\medskip
\noindent {\bf Solution:}
\begin{align*}
\frac{dy}{dx}(t^3\ln t) &= 3t^2\ln t + t^3\frac{1}{t}\\
&= 3t^2\ln t + t^2 \\
&= t^2(3\ln t + 1)
\end{align*}

\bigskip

\newpage
%=======================================================================

\noindent Midterm Exam \hfill page 2

\item Find
\[
\lim_{x\rightarrow 1^-} \frac{x^2 + 4x + 3}{x^2 - 1}
\]

\medskip
\noindent {\bf Solution:}
%% \begin{align*}
%% \lim_{x\rightarrow 1^-} \frac{x^2 + 4x + 3}{x^2 - 1}&=\lim_{x\rightarrow 1^-} \frac{(x+1)(x+3)}{(x+1)(x-1)}\\
%% &=\lim_{x\rightarrow 1^-} \frac{x+3}{x-1}\\ 
%% &=-\infty
%% \end{align*}
\[
\lim_{x\rightarrow 1^-} \frac{x^2 + 4x + 3}{x^2 - 1}=\lim_{x\rightarrow 1^-} \frac{(x+1)(x+3)}{(x+1)(x-1)}
=\lim_{x\rightarrow 1^-} \frac{x+3}{x-1}\\ 
=-\infty
\]

\bigskip

\item Let
\[
y = \frac{3x^2 - 5x - 2}{x^2 - 4}.
\]
Give the equations of all the horizontal asymptotes.

\medskip
\noindent {\bf Solution:}
%% \begin{align*}
%% \lim_{x\rightarrow \infty} \frac{3x^2 - 5x - 2}{x^2 - 4} &=
%% \lim_{x\rightarrow \infty} \frac{3 - 5/x - 2/x^2}{1 - 4/x^2}\\ &=
%% \frac{3-0-0}{1-0}\\
%%  &=3
%% \end{align*}
\[
\lim_{x\rightarrow \infty} \frac{3x^2 - 5x - 2}{x^2 - 4} =
\lim_{x\rightarrow \infty} \frac{3 - 5/x - 2/x^2}{1 - 4/x^2} =
\frac{3-0-0}{1-0}
=3
\]
Therefore $y = 3$ is the horizontal asymptote.

\bigskip

\item Let
\[
y = \frac{3x^2 - 5x - 2}{x^2 - 4}
\]
Give the equations of all the vertical asymptotes.

\medskip
\noindent {\bf Solution:}
%% \begin{align*}
%% y = \frac{3x^2 - 5x - 2}{x^2 - 4} &= \frac{(x-2)(3x+1)}{(x-2)(x+2)}\\
%% &=\frac{3x+1}{x+2}
%% \end{align*}
\[
y = \frac{3x^2 - 5x - 2}{x^2 - 4} = \frac{(x-2)(3x+1)}{(x-2)(x+2)}
=\frac{3x+1}{x+2}
\]
The function is not defined when the denominator is 0, therefore, $x = -2$ is
the vertical asymptote. 
\bigskip

\newpage

\noindent Midterm Exam \hfill page 3

\item Find the derivative of $4x^3 \tan^2(x)$. 
You do not need to simplify your answer.

\medskip
\noindent {\bf Solution:}

\begin{align*}
\frac{dy}{dx}(4x^3\tan^2(x)) &= 12x^2\tan^2(x) + 4x^3
\frac{dy}{dx}\tan^2(x)\\
&= 12x^2\tan^2(x) + 4x^3(2\tan(x)\sec^2(x))\\
\end{align*}

\bigskip

\item Find the slope of the line tangent to the graph of 
$y = \sqrt{x^2 + 4x - 5}$ at $x = 3$. Simplify your answer.

\medskip
\noindent {\bf Solution:}
\[
y' = f'(x) = (1/2)(x^2 + 4x - 5)^{-1/2}(2x + 4),
\]
so the slope at $x = 3$ is
\[
f'(3) = (1/2)(3^2 + 4(3) - 5)^{-1/2}(2(3) + 4)
= \frac{10}{2\sqrt{16}}
= \frac{5}{4}.
\]
\bigskip

\item Suppose $f(x) = \sin^4(3e^x + 1)$. Find $f'(x)$. 
You do not need to simplify your answer.

\medskip
\noindent {\bf Solution:}
\begin{align*}
f'(x) &= 4\sin^3(3e^x+1)\frac{dy}{dx}\sin(3e^x+1)\\
&= 4\sin^3(3e^x+1)\cos(3e^x+1)\frac{dy}{dx}(3e^x+1)\\
&= 4\sin^3(3e^x+1)\cos(3e^x+1)3e^x\\
\end{align*}

\bigskip

\item Let $f(x) = x^3 + 2x^2 + 1$ for $x \geq 0$. 
Using that $f(1) = 4$, find $(f^{-1})'(4)$.

\medskip
\noindent {\bf Solution:}
\begin{align*}
(f^{-1})'(y) &= \frac{1}{f'(f^{-1}(y))}\\
&= \frac{1}{3(f^{-1}(y))^2 + 4f^{-1}(y)}
\end{align*}
Since $f^{-1}(4) = 1$,
\[
(f^{-1})'(4) = \frac{1}{3 + 4}.
= \frac{1}{7} 
\]
\end{enumerate}

\end{document}
